Scoping is not changed by the evaluation

src/CTX.v
@@ -2,11 +2,23 @@ Require Import LogRel.
 
 Import ListNotations.
 
+Check fold_left.
+
+Theorem fold_left_map :
+  forall (T T2 T3 : Type) (l : list T) f (f2 : T -> T2 -> T3 -> T) d t2 t3,
+  (forall a b t2 t3, f2 (f a b) t2 t3 = f (f2 a t2 t3) (f2 b t2 t3)) ->
+  f2 (fold_left f l d) t2 t3 = fold_left f (map (fun x => f2 x t2 t3) l) (f2 d t2 t3).
+Proof.
+  induction l; intros; auto.
+  intros. cbn.
+  rewrite IHl; auto. rewrite H. auto.
+Qed.
+
 Definition Adequate (R : list VarFunId -> Exp -> Exp -> Prop) :=
   forall e1 e2,
     R [] e1 e2 ->
-    forall v1 v2, equivalent_values v1 v2 -> (exists clock, eval clock e1 = Res v1) <-> 
-                                             (exists clock, eval clock e2 = Res v2).
+    forall v1, (exists clock, eval clock e1 = Res v1) ->
+         exists v2, (exists clock, eval clock e2 = Res v2) /\ equivalent_values v1 v2.
 
 Definition IsReflexive (R : list VarFunId -> Exp -> Exp -> Prop) :=
   forall Γ e,
@@ -65,6 +77,47 @@ Definition IsCtxRel (R : list VarFunId -> Exp -> Exp -> Prop) :=
   IsPreCtxRel R /\
   forall R', IsPreCtxRel R' ->
     forall Γ e1 e2, R' Γ e1 e2 -> R Γ e1 e2.
+
+(* Lemma CTX_closed_under_substitution : forall {Γ e1 e2 vals CTX},
+    IsCtxRel CTX ->
+    Forall (fun v => VAL Γ ⊢ v) vals ->
+    CTX (Γ ++ l) e1 e2 ->
+    CTX Γ (subst ξ e1) (subst ξ e2).
+Proof.
+  intros Γ e1 e2 v CTX HCtx Hscope_v HCtx_e1e2.
+  destruct HCtx as [HCtx Hbiggest].
+  destruct HCtx as [Rscope [Radequate [Rrefl [Rtrans [RFun [RApp [RSeq RFactor]]]]]]].
+  destruct (Rscope _ _ _ HCtx_e1e2) as [Hscope_e1 Hscope_e2].
+  pose proof (CIU_beta_value Hscope_e1 Hscope_v).
+  pose proof (CIU_beta_value Hscope_e2 Hscope_v).
+  destruct H as [? _].
+  destruct H0 as [_ ?].
+  apply CIU_iff_Erel in H.
+  apply CIU_iff_Erel in H0.
+  apply Hbiggest in H; auto using Erel_IsPreCtxRel.
+  apply Hbiggest in H0; auto using Erel_IsPreCtxRel.
+  eapply Rtrans in H.
+  eapply H.
+  eapply Rtrans; revgoals.
+  eapply H0.
+  auto.
+Qed. *)
+
+Lemma bigger_implies_IsCtxRel : forall E R,
+    IsCtxRel R ->
+    IsPreCtxRel E ->
+    (forall Γ e1 e2, R Γ e1 e2 -> E Γ e1 e2) ->
+    IsCtxRel E.
+Proof.
+  intros.
+  split; auto.
+  intros.
+  apply H1.
+  destruct H.
+  eapply H4.
+  - exact H2.
+  - auto.
+Qed.
 
 Inductive Ctx :=
 | CHole
@@ -272,8 +325,9 @@ Qed.
 Definition CTX (Γ : list VarFunId) (e1 e2 : Exp) :=
   (EXP Γ ⊢ e1 /\ EXP Γ ⊢ e2) /\
   (forall (C : Ctx),
-      EECTX Γ ⊢ C ;; [] -> forall v1 v2, equivalent_values v1 v2 ->
-      (exists clock, eval clock (plug C e1) = Res v1) <-> (exists clock, eval clock (plug C e2) = Res v2)).
+      EECTX Γ ⊢ C ;; [] -> forall v1,
+      (exists clock, eval clock (plug C e1) = Res v1) -> 
+      exists v2, (exists clock, eval clock (plug C e2) = Res v2) /\ equivalent_values v1 v2).
 
 Lemma IsReflexiveList : forall R' l Γ',
   IsReflexive R' -> Forall (fun v : Exp => EXP Γ' ⊢ v) l ->
@@ -398,6 +452,339 @@ Proof.
         simpl in H0. inversion H0. auto. inversion H1.
   }
   apply H1.
-  auto.
-Unshelve. exact (ELit 0).
+  auto. Grab Existential Variables. exact (ELit 0).
 Qed.
+
+Lemma CTX_refl Γ e : EXP Γ ⊢ e -> CTX Γ e e.
+Proof.
+  unfold CTX. intros. split; auto.
+  intros. intuition. destruct H1. exists v1. split. eexists. eauto.
+  exists 0. eapply Vrel_Fundamental_closed.
+  
+Qed.
+
+Lemma CTX_IsPreCtxRel : IsPreCtxRel CTX.
+Proof.
+  unfold IsPreCtxRel.
+  intuition idtac;
+    try solve
+        [unfold CTX in H; intuition idtac
+        |inversion H; [|constructor]; apply H0].
+  * unfold Adequate.
+    intros.
+    unfold CTX in H.
+    intuition idtac.
+    + eapply (H2 CHole); eauto.
+      constructor.
+    + eapply (H2 CHole); eauto.
+      constructor.
+  * unfold IsReflexive.
+    intros.
+    unfold CTX.
+    
+  - unfold Transitive.
+    intros.
+    unfold CTX in *.
+    intuition idtac.
+    eapply Rbar_le_trans; firstorder.
+  - unfold CompatibleFun.
+    intros.
+    unfold CTX in *.
+    intuition auto.
+    specialize (H1 (plugc C (Ctx_Fun Ctx_hole)) A).
+    repeat rewrite <- plug_assoc in H1.
+    cbn in H1.
+    apply H1.
+    eapply plugc_preserves_scope_exp; eauto.
+    repeat constructor.
+  - unfold CompatibleApp.
+    intros.
+    unfold CTX in *.
+    intuition auto.
+    assert (EECTX Γ ⊢ plugc C (Ctx_Seq_x Ctx_hole (App (Var 0) (rename (+1) v1))) ∷ 0).
+    { eapply plugc_preserves_scope_exp; eauto.
+      constructor.
+      constructor.
+      constructor.
+      constructor.
+      auto.
+      apply -> ren_preserves_scope_val; eauto.
+      unfold RenScoped.
+      intros; asimpl; auto.
+    }
+    specialize (H6 _ A H10).
+    repeat rewrite <- plug_assoc in H6.
+    cbn in H6.
+    assert (forall f1 v1,
+               VAL Γ ⊢ f1 ->
+               VAL Γ ⊢ v1 ->
+               (μeval_star (plug C (App f1 v1)) Knil A =
+                μeval_star (plug C (Seq f1 (App (Var 0) (rename (+1) v1)))) Knil A))
+      as HApp_Seq_f.
+    { intros.
+      erewrite use_Seq_instead; eauto 2.
+      asimpl.
+      reflexivity.
+      constructor; auto.
+      apply -> ren_preserves_scope_val; eauto.
+      unfold RenScoped.
+      intros; cbn; auto.
+    }
+    assert (forall f1 v1,
+               VAL Γ ⊢ f1 ->
+               VAL Γ ⊢ v1 ->
+               (μeval_star (plug C (App f1 v1)) Knil A =
+                μeval_star (plug C (Seq v1 (App (rename (+1) f1) (Var 0)))) Knil A))
+      as HApp_Seq_v.
+    { intros.
+      erewrite use_Seq_instead; eauto 2.
+      asimpl.
+      reflexivity.
+      constructor; auto.
+      apply -> ren_preserves_scope_val; eauto.
+      unfold RenScoped.
+      intros; cbn; auto.
+    }
+    rewrite HApp_Seq_f; auto.
+    eapply Rbar_le_trans.
+    apply H6.
+    assert (EECTX Γ ⊢ plugc C (Ctx_Seq_x Ctx_hole (App (rename (+1) f2) (Var 0))) ∷ 0).
+    { eapply plugc_preserves_scope_exp; eauto.
+      constructor.
+      constructor.
+      constructor.
+      - apply -> ren_preserves_scope_val; eauto.
+        unfold RenScoped.
+        intros; asimpl; auto.
+      - constructor.
+        auto.
+    }
+    specialize (H7 _ A H11).
+    repeat rewrite <- plug_assoc in H7.
+    rewrite HApp_Seq_v; auto.
+    eapply Rbar_le_trans; revgoals.
+    cbn in H7.
+    apply H7.
+    rewrite <- HApp_Seq_v; auto.
+    rewrite <- HApp_Seq_f; auto.
+  - unfold CompatibleOp1.
+    intros.
+    unfold CTX in *.
+    intuition auto.
+    assert (EECTX Γ ⊢ plugc C (Ctx_Seq_x Ctx_hole (Op1 o (Var 0))) ∷ 0).
+    { eapply plugc_preserves_scope_exp; eauto.
+      constructor.
+      constructor.
+      constructor.
+      constructor.
+      auto.
+    }
+    specialize (H3 _ A H5).
+    repeat rewrite <- plug_assoc in H3.
+    cbn in H3.
+    assert (forall v1,
+               VAL Γ ⊢ v1 ->
+               (μeval_star (plug C (Op1 o v1)) Knil A =
+                μeval_star (plug C (Seq v1 (Op1 o (Var 0)))) Knil A))
+      as HApp_Op1.
+    { intros.
+      erewrite use_Seq_instead; eauto 2.
+      constructor.
+      auto.
+    }
+    rewrite HApp_Op1; auto.
+    eapply Rbar_le_trans.
+    apply H3.
+    rewrite HApp_Op1; auto.
+  - unfold CompatibleOp2.
+    intros.
+    unfold CTX in *.
+    intuition auto.
+    assert (EECTX Γ ⊢ plugc C (Ctx_Seq_x Ctx_hole (Op2 o (Var 0) (rename (+1) v1'))) ∷ 0).
+    { eapply plugc_preserves_scope_exp;
+        eauto;
+        repeat (constructor; auto 1).
+      apply -> ren_preserves_scope_val;
+        eauto.
+      unfold RenScoped.
+      cbn.
+      auto.
+    }
+    specialize (H6 _ A H10).
+    repeat rewrite <- plug_assoc in H6.
+    cbn in H6.
+    assert (forall v1,
+               VAL Γ ⊢ v1 ->
+               (μeval_star (plug C (Op2 o v1 v1')) Knil A =
+                μeval_star (plug C (Seq v1 (Op2 o (Var 0) (rename (+1) v1')))) Knil A))
+      as HApp_Op2_1.
+    { intros.
+      erewrite use_Seq_instead; eauto 2.
+      asimpl.
+      auto.
+      constructor.
+      - auto.
+      - apply -> ren_preserves_scope_val; eauto.
+        unfold RenScoped.
+        cbn.
+        auto.
+    }
+    assert (forall v1',
+               VAL Γ ⊢ v1' ->
+               (μeval_star (plug C (Op2 o v2 v1')) Knil A =
+                μeval_star (plug C (Seq v1' (Op2 o (rename (+1) v2) (Var 0)))) Knil A))
+      as HApp_Op2_2.
+    { intros.
+      erewrite use_Seq_instead; eauto 2.
+      asimpl.
+      auto.
+      constructor.
+      - apply -> ren_preserves_scope_val; eauto.
+        unfold RenScoped.
+        cbn.
+        auto.
+      - auto.
+    }
+    rewrite HApp_Op2_1; auto.
+    eapply Rbar_le_trans.
+    apply H6.
+    assert (EECTX Γ ⊢ plugc C (Ctx_Seq_x Ctx_hole (Op2 o (rename (+1) v2) (Var 0))) ∷ 0).
+    { eapply plugc_preserves_scope_exp; eauto.
+      constructor.
+      constructor.
+      constructor.
+      - apply -> ren_preserves_scope_val; eauto.
+        unfold RenScoped.
+        intros; asimpl; auto.
+      - constructor.
+        auto.
+    }
+    specialize (H7 _ A H11).
+    repeat rewrite <- plug_assoc in H7.
+    rewrite HApp_Op2_2; auto.
+    eapply Rbar_le_trans; revgoals.
+    cbn in H7.
+    apply H7.
+    rewrite <- HApp_Op2_2; auto.
+    rewrite <- HApp_Op2_1; auto.
+  - unfold CompatibleCond.
+    intros.
+    unfold CTX in *.
+    intuition auto.
+    assert (EECTX Γ ⊢ plugc C (Ctx_Cond_t v1 Ctx_hole ef1) ∷ 0) as HCtx_t.
+    { eapply plugc_preserves_scope_exp; eauto.
+      constructor; auto.
+      constructor.
+    }
+    assert (EECTX Γ ⊢ plugc C (Ctx_Cond_f v1 et2 Ctx_hole) ∷ 0) as HCtx_f.
+    { eapply plugc_preserves_scope_exp; eauto.
+      constructor; auto.
+      constructor.
+    }
+    specialize (H10 _ A HCtx_t).
+    repeat rewrite <- plug_assoc in H10.
+    cbn in H10.
+    eapply Rbar_le_trans.
+    apply H10.
+    specialize (H11 _ A HCtx_f).
+    repeat rewrite <- plug_assoc in H11.
+    cbn in H11.
+    eapply Rbar_le_trans.
+    apply H11.
+    assert (EECTX Γ ⊢ plugc C (Ctx_Seq_x Ctx_hole (Cond (Var 0) (rename (+1) et2) (rename (+1) ef2))) ∷ 0) as HCtx_p.
+    { eapply plugc_preserves_scope_exp;
+        eauto.
+      constructor.
+      constructor.
+      constructor.
+      + constructor.
+        auto.
+      + apply -> ren_preserves_scope_exp;
+          eauto.
+        unfold RenScoped.
+        cbn.
+        auto 1.
+      + apply -> ren_preserves_scope_exp;
+          eauto.
+        unfold RenScoped.
+        cbn.
+        auto 1.
+    }
+    specialize (H9 _ A HCtx_p).
+    repeat rewrite <- plug_assoc in H9.
+    cbn in H9.
+    assert (forall vp,
+               VAL Γ ⊢ vp ->
+               (μeval_star (plug C (Cond vp et2 ef2)) Knil A =
+                μeval_star (plug C (Seq vp (Cond (Var 0) (rename (+1) et2) (rename (+1) ef2)))) Knil A))
+      as HSeq_Cond_p.
+    { intros.
+      erewrite use_Seq_instead; eauto 2.
+      asimpl.
+      auto.
+      constructor.
+      - auto.
+      - apply -> ren_preserves_scope_exp; eauto.
+        unfold RenScoped.
+        cbn.
+        auto 1.
+      - apply -> ren_preserves_scope_exp; eauto.
+        unfold RenScoped.
+        cbn.
+        auto 1.
+    }
+    rewrite HSeq_Cond_p; auto.
+    eapply Rbar_le_trans.
+    apply H9.
+    rewrite <- HSeq_Cond_p; auto.
+  - unfold CompatibleSeq.
+    intros.
+    unfold CTX in *.
+    intuition auto.
+    assert (EECTX Γ ⊢ (plugc C (Ctx_Seq_x Ctx_hole b1)) ∷ 0).
+    { eapply plugc_preserves_scope_exp; eauto.
+      constructor.
+      constructor.
+      auto.
+    }
+    specialize (H2 _ A H6).
+    repeat rewrite <- plug_assoc in H2.
+    cbn in H2.
+    eapply Rbar_le_trans.
+    eapply H2.
+    assert (EECTX S Γ ⊢ (plugc C (Ctx_Seq_b x2 Ctx_hole)) ∷ 0).
+    { eapply plugc_preserves_scope_exp; eauto.
+      constructor.
+      auto.
+      constructor.
+    }
+    specialize (H3 _ A H7).
+    repeat rewrite <- plug_assoc in H3.
+    cbn in H3.
+    apply H3.
+  - unfold CompatibleFactor.
+    intros.
+    unfold CTX in *.
+    intuition auto.
+    assert (EECTX Γ ⊢ (plugc C (Ctx_Seq_x Ctx_hole (Factor (Var 0)))) ∷ 0).
+    { eapply plugc_preserves_scope_exp; eauto.
+      constructor.
+      constructor.
+      auto.
+    }
+    specialize (H3 _ A H5).
+    repeat rewrite <- plug_assoc in H3.
+    cbn in H3.
+    assert (forall v1,
+               VAL Γ ⊢ v1 ->
+               (μeval_star (plug C (Factor v1)) Knil A =
+                μeval_star (plug C (Seq v1 (Factor (Var 0)))) Knil A))
+      as HFactor_Seq.
+    { intros.
+      erewrite use_Seq_instead; eauto 2.
+      auto.
+    }
+    rewrite HFactor_Seq; auto.
+    rewrite HFactor_Seq; auto.
+Qed.
+
